Start working on bank example

src/Dafny/bank.dfy
@@ -3,3 +3,33 @@ include "jrnl.i.dfy"
 /*
 Demo of bank transfer using axiomatized journal API
 */
+class Bank {
+    var jrnl: Jrnl;
+    constructor(jrnl: Jrnl)
+    requires jrnl.Valid()
+    ensures this.Valid()
+    {
+        this.jrnl := jrnl;
+    }
+
+    predicate Valid()
+    reads {this,this.jrnl} + this.jrnl.Repr
+    {
+        this.jrnl.Valid()
+    }
+
+    method transfer(acct1: Addr, acct2: Addr, sz: nat)
+    requires Valid()
+    requires acct1 in jrnl.domain()
+    requires acct2 in jrnl.domain()
+    requires jrnl.size(acct1) == sz
+    requires jrnl.size(acct2) == sz
+    modifies {this.jrnl} + this.jrnl.Repr
+    {
+        assert acct1 in jrnl.domain();
+        var txn := jrnl.Begin();
+        var x := txn.Read(acct1, sz);
+        txn.Write(acct2, x);
+        txn.Commit();
+    }
+}
